New benchmakrs. Bug fixes. Incremental if-conditionals in grammar added. Constants in comparison modelled as variables to enable bounded checking. All benchmakrs synthesize correctly. Benchmarks with conditionals don't pass dafny yet. New flags added for sketch.

bin/benchmarks/Average.java
@@ -1,9 +1,11 @@
 import java.util.List;
+import java.util.Arrays;
 import java.lang.Integer;
 
 public class Average {	
 	public static void main(String[] args) {
-		avgList(null);
+		List<Integer> numbers = Arrays.asList(10, 5, 7, 12, 3);
+		avgList(numbers);
 	}
 	
 	public static int avgList(List<Integer> data) {
