bin/benchmarks/Equal.java
@@ -1,9 +1,11 @@
 import java.util.List;
+import java.util.Arrays;
 import java.lang.Integer;
 
 public class Equal {	
 	public static void main(String[] args) {
-		equal(null);
+		List<Integer> numbers = Arrays.asList(10, 10, 5, 10, 10);
+		equal(numbers);
 	}
 	
 	public static boolean equal(List<Integer> data) {
