bin/benchmarks/WordCount.java
@@ -1,12 +1,16 @@
 import java.util.List;
+import java.util.Arrays;
 import java.util.Map;
+import java.util.HashMap;
 import java.lang.Integer;
 import java.lang.String;
 
 public class WordCountJava {
 
 	public static void main(String[] args) {
-		countWords(null, null);
+		List<String> words = Arrays.asList("foo", "bar", "cat", "bar", "dog");
+		Map<String, Integer> counts = new HashMap<String, Integer>();
+		countWords(words, counts);
 	}
 
 	private static Map<String, Integer> countWords(List<String> words, Map<String, Integer> counts) {
